msl/log_normalize.v
@@ -1,0 +1,874 @@
+Require Import msl.seplog.
+Require Import msl.alg_seplog.
+Require Import msl.Extensionality.
+
+Local Open Scope logic.
+
+Hint Resolve @derives_refl.
+
+
+Lemma TT_right {A}{NA: NatDed A}: forall P:A, P |-- TT.
+Proof. intros; apply prop_right; auto.
+Qed.
+
+Hint Resolve @TT_right: normalize.
+
+Ltac norm := auto with normalize.
+
+Lemma andp_dup {A}{ND: NatDed A}: forall P: A, P && P = P.
+Proof. intros. apply pred_ext.
+apply andp_left1; apply derives_refl.
+apply andp_right; apply derives_refl.
+Qed.
+
+
+Lemma FF_left {A}{NA: NatDed A}: forall P, FF |-- P.
+Proof.
+intros; apply prop_left. intuition.
+Qed.
+Hint Resolve @FF_left : normalize.
+
+Lemma andp_TT {A}{NA: NatDed A}: forall (P: A), P && TT = P.
+Proof with norm.
+intros.
+apply pred_ext.
+apply andp_left1...
+apply andp_right...
+Qed.
+
+Lemma sepcon_andp_prop'  {A}{NA: NatDed A}{SA: SepLog A}: 
+     forall P Q R, (!!Q && P)*R = !!Q&&(P*R).
+Proof with norm.
+intros.
+rewrite sepcon_comm. rewrite sepcon_andp_prop.
+rewrite sepcon_comm; auto.
+Qed.
+
+Lemma emp_sepcon  {A}{NA: NatDed A}{SA: SepLog A}{CA: ClassicalSep A} : forall (P:A),
+   emp * P = P.
+Proof with norm.
+ intros; rewrite sepcon_comm. apply sepcon_emp.
+Qed.
+
+Lemma TT_andp {A}{NA: NatDed A}: forall P: A,  TT && P = P.
+Proof with norm.
+  intros. apply pred_ext. apply andp_left2... apply andp_right...
+Qed.
+
+Lemma exp_sepcon2 {A}{NA: NatDed A}{SA: SepLog A}: 
+   forall T (P: A) (Q: T -> A),  P * exp Q = exp (fun x => P * Q x).
+Proof. intros.
+ rewrite sepcon_comm. rewrite exp_sepcon1.
+ f_equal. extensionality x. apply sepcon_comm.
+Qed.
+
+Lemma andp_com  {A}{NA: NatDed A}:
+  forall P Q,  P && Q = Q && P.
+Proof with norm.
+ intros.
+   apply pred_ext.
+   apply andp_right. apply andp_left2... apply andp_left1...
+    apply andp_right. apply andp_left2... apply andp_left1...
+Qed.
+
+Lemma andp_assoc {A} {NA: NatDed A} : forall P Q R,
+  (P && Q) && R = P && (Q && R).
+Proof.
+  intros; apply pred_ext;   repeat apply andp_right.
+  do 2 apply andp_left1; auto.
+  apply andp_left1; apply andp_left2; auto.
+  apply andp_left2; auto.
+  apply andp_left1; auto.
+  apply andp_left2; apply andp_left1; auto.
+  do 2 apply andp_left2; auto.
+Qed.
+
+Lemma exp_andp2  {A}{NA: NatDed A}:
+ forall B (p: A) (q: B -> A) , (p && exp q) = exp (fun x => p && q x).
+Proof.
+ intros. rewrite andp_com; rewrite exp_andp1.
+ f_equal. extensionality x. apply andp_com.
+Qed.
+
+Hint Rewrite @sepcon_emp @emp_sepcon @TT_andp @andp_TT 
+             @exp_sepcon1 @exp_sepcon2
+               @exp_andp1 @exp_andp2
+         @sepcon_andp_prop @sepcon_andp_prop'
+        : normalize.
+
+
+Lemma andp_derives {A} {NA: NatDed A}:
+  forall P Q P' Q': A, P |-- P' -> Q |-- Q' -> P && Q |-- P' && Q'.
+Proof.
+intros.
+apply andp_right.
+eapply derives_trans; try apply H.
+apply andp_left1; auto.
+eapply derives_trans; try apply H0.
+apply andp_left2; auto.
+Qed.
+
+Lemma imp_derives {A} {NA: NatDed A}:
+  forall P P' Q Q',
+    P' |-- P ->
+    Q |-- Q' -> 
+    P --> Q |-- P' --> Q'.
+Proof.
+intros.
+apply imp_andp_adjoint. 
+eapply derives_trans; try apply H0; clear H0.
+eapply derives_trans; [ apply andp_derives; try apply H | ]; clear H.
+apply derives_refl.
+rewrite andp_com. apply modus_ponens.
+Qed.
+
+Lemma pure_sepcon {A}{NA: NatDed A}{SA: SepLog A}{CA: ClassicalSep A}:
+    forall (P : A), pure P -> P*P=P.
+Proof with norm.
+ intros. pose proof (sepcon_pure_andp _ _ H H).
+ rewrite H0. apply pred_ext. apply andp_left1... apply andp_right...
+Qed.
+
+Lemma pure_e  {A}{NA: NatDed A}{SA: SepLog A}: forall (P: A), pure P -> (P |-- emp).
+Proof.
+intros.
+apply H.
+Qed.
+
+Hint Resolve @pure_e : normalize.
+
+Lemma pure_emp {A}{NA: NatDed A}{SA: SepLog A}: pure emp.
+Proof with norm.
+intros. unfold pure...
+Qed.
+Hint Resolve @pure_emp.
+
+Lemma pure_sepcon1''  {A}{NA: NatDed A}{SA: SepLog A}{CA: ClassicalSep A}: 
+   forall P Q R, pure P -> Q |-- R -> P * Q |-- R.
+Proof with norm.
+intros.
+apply @derives_trans with (emp*Q).
+apply sepcon_derives...
+rewrite emp_sepcon...
+Qed.
+
+
+Lemma pure_existential {A}{NA: NatDed A}{SA: SepLog A}{CA: ClassicalSep A}:
+   forall B (P: B -> A),    (forall x: B , pure (P x)) -> pure (exp P).
+Proof.
+intros.
+unfold pure in *.
+apply exp_left; auto.
+Qed.
+
+Hint Resolve @pure_existential.
+
+Lemma FF_sepcon {A} {NA: NatDed A}{SA: SepLog A}: forall P, FF * P = FF.
+Proof.
+intros.
+rewrite sepcon_comm. apply sepcon_FF.
+Qed.
+
+Hint Rewrite @FF_sepcon @sepcon_FF : normalize.
+
+Lemma prop_true_andp {A} {NA: NatDed A}:
+  forall (P: Prop) Q,  P -> (!! P && Q = Q).
+Proof with norm.
+intros.
+apply pred_ext. apply andp_left2...
+apply andp_right... apply prop_right...
+Qed.
+
+Hint Rewrite @prop_true_andp using (solve [auto]) : normalize.
+
+Lemma true_eq {A} {NA: NatDed A}:  forall P: Prop, P -> (!! P) = (TT: A).
+Proof with norm.
+intros. apply pred_ext...
+apply prop_right...
+Qed. 
+Hint Rewrite @true_eq using (solve [auto]) : normalize.
+
+Lemma pure_con' {A}{NA: NatDed A}{SA: SepLog A}{CA: ClassicalSep A}: 
+      forall P Q, pure P -> pure Q -> pure (P*Q).
+Proof.
+intros.
+unfold pure in *.
+rewrite <- sepcon_emp.
+apply sepcon_derives; auto.
+Qed.
+Hint Resolve @pure_con'.
+
+Lemma pure_intersection1: forall {A}{NA: NatDed A}{SA: SepLog A}{CA: ClassicalSep A}
+       (P Q: A), pure P -> pure (P && Q).
+Proof.
+unfold pure; intros; auto.
+apply andp_left1; auto.
+Qed.
+
+Lemma pure_intersection2: forall {A}{NA: NatDed A}{SA: SepLog A}{CA: ClassicalSep A}
+     (P Q: A), pure Q -> pure (P && Q).
+Proof.
+unfold pure; intros; auto.
+apply andp_left2; auto.
+Qed.
+Hint Resolve @pure_intersection1 @pure_intersection2.
+
+Lemma FF_andp {A}{NA: NatDed A}:  forall P: A, FF && P = FF.
+Proof with norm.
+intros. apply pred_ext...
+apply andp_left1...
+Qed.
+
+Lemma andp_FF {A}{NA: NatDed A}:  forall P: A, P && FF = FF.
+Proof.
+intros. rewrite andp_com. apply FF_andp.
+Qed.
+Hint Rewrite @FF_andp @andp_FF : normalize.
+
+Hint Rewrite @andp_dup : normalize.
+
+Lemma sepcon_TT {A} {NA: NatDed A}{SA: SepLog A}{CA: ClassicalSep A}:
+   forall (P: A), P |-- (P * TT).
+Proof with norm.
+intros.
+apply @derives_trans with (P * emp).
+rewrite sepcon_emp...
+apply sepcon_derives...
+Qed.
+Hint Resolve @sepcon_TT.
+
+Lemma imp_extract_exp_left {B A: Type} {NA: NatDed A}:
+    forall    (p : B -> A) (q: A),
+  (forall x, p x |-- q) ->
+   exp p |-- q.
+Proof.
+intros.
+apply exp_left. auto.
+Qed.
+
+Lemma allp_derives: 
+       forall {A: Type}  {NA: NatDed A} (B: Type) (P Q: B -> A), 
+               (forall x:B, P x |-- Q x) -> (allp P |-- allp Q).
+Proof.
+intros.
+apply allp_right; intro x; apply allp_left with x; auto.
+Qed.
+
+Lemma forall_pred_ext  {A}  {NA: NatDed A}: forall B (P Q: B -> A), 
+ (All x : B, (P x <--> Q x)) |-- (All x : B, P x) <--> (All x: B, Q x) .
+Proof.
+intros.
+apply andp_right.
+ apply @derives_trans with (All x:B, P x --> Q x).
+ apply allp_derives; intro x; apply andp_left1; auto.
+ apply imp_andp_adjoint; apply allp_right; intro x.
+ apply @derives_trans with ((P x --> Q x) && P x).
+ apply andp_derives; apply allp_left with x; auto.
+ rewrite andp_com. apply modus_ponens.
+ apply @derives_trans with (All x:B, Q x --> P x).
+ apply allp_derives; intro x; apply andp_left2; auto.
+ apply imp_andp_adjoint; apply allp_right; intro x.
+ apply @derives_trans with ((Q x --> P x) && Q x).
+ apply andp_derives; apply allp_left with x; auto.
+ rewrite andp_com. apply modus_ponens.
+Qed.
+
+Lemma exists_pred_ext  {A} {NA: NatDed A}: forall B (P Q: B -> A), 
+ (All x : B, (P x <--> Q x)) |-- (Ex x : B, P x) <--> (Ex x: B, Q x) .
+Proof.
+intros.
+apply andp_right.
+ apply imp_andp_adjoint.
+autorewrite with normalize.
+apply exp_left; intro x. apply exp_right with x.
+ apply imp_andp_adjoint.
+apply allp_left with x. apply andp_left1; auto.
+ apply imp_andp_adjoint.
+autorewrite with normalize.
+apply exp_left; intro x. apply exp_right with x.
+ apply imp_andp_adjoint.
+apply allp_left with x. apply andp_left2; auto.
+Qed.
+
+Lemma imp_pred_ext  {A}  {NA: NatDed A}: forall B B' P Q, 
+       (B <--> B') && (B --> (P <--> Q)) 
+ |-- (B --> P) <-->  (B' --> Q).
+Proof.
+intros.
+apply andp_right.
+apply -> imp_andp_adjoint.
+apply -> imp_andp_adjoint.
+rewrite andp_com.
+rewrite (andp_com (B --> B')).
+repeat rewrite <- andp_assoc.
+do 2 rewrite andp_assoc.
+eapply derives_trans; [eapply andp_derives; [apply modus_ponens | apply derives_refl] | ].
+apply @derives_trans with ((B && (B --> (P --> Q))) && (B && (B --> P))).
+repeat apply andp_right.
+apply andp_left1; auto.
+apply andp_left2. apply andp_left2. apply andp_left1. apply imp_derives; auto.
+apply andp_left1; auto.
+apply andp_left1; auto.
+apply andp_left2. apply andp_left2. apply andp_left2. auto.
+apply @derives_trans with ((P --> Q) && P).
+apply andp_derives; apply modus_ponens.
+rewrite andp_com; apply modus_ponens.
+apply -> imp_andp_adjoint.
+apply -> imp_andp_adjoint.
+rewrite andp_com.
+repeat rewrite <- andp_assoc.
+do 2 rewrite andp_assoc.
+eapply derives_trans; [eapply andp_derives; [apply modus_ponens | apply derives_refl] | ].
+apply @derives_trans with ((B' && (B' --> (Q --> P))) && (B' && (B' --> Q))).
+repeat apply andp_right.
+apply andp_left1; auto.
+repeat rewrite <- andp_assoc.
+apply andp_left1.
+apply -> imp_andp_adjoint.
+apply andp_left1.
+eapply derives_trans; [eapply andp_derives; [apply modus_ponens | apply derives_refl] | ].
+eapply derives_trans; [apply modus_ponens | ].
+apply andp_left2; auto.
+apply andp_left1; auto.
+repeat apply andp_left2. auto.
+eapply derives_trans; [eapply andp_derives; apply modus_ponens | ].
+rewrite andp_com; apply modus_ponens.
+Qed.
+
+Lemma pure_sepcon_TT_andp'  {A} {NA: NatDed A}{SA: SepLog A}{CA: ClassicalSep A}:
+  forall P Q, pure P -> Q && (P * TT) = (Q*P).
+Proof.
+intros. rewrite andp_com.
+rewrite pure_sepcon_TT_andp; auto.
+apply sepcon_comm.
+Qed.
+
+Hint Rewrite @pure_sepcon_TT_andp @pure_sepcon_TT_andp' using (solve [auto]): normalize.
+
+Lemma pure_sepcon1'  {A} {NA: NatDed A}{SA: SepLog A}{CA: ClassicalSep A}:
+  forall P Q R, pure P -> P * Q |-- P * R -> P * Q |-- R.
+Proof with norm.
+intros.
+eapply derives_trans; try apply H0.
+apply pure_sepcon1''; auto.
+Qed.
+
+Lemma pull_right {A} {NA: NatDed A}{SA: SepLog A}:
+ forall P Q R,
+   (Q * P * R) = (Q * R * P).
+Proof.
+intros. repeat rewrite sepcon_assoc. rewrite (sepcon_comm P); auto.
+Qed.
+
+Lemma pull_right0 {A} {NA: NatDed A}{SA: SepLog A}:
+  forall P Q,   (P * Q) = (Q * P).
+Proof.
+intros. rewrite (sepcon_comm P); auto.
+Qed.
+
+Ltac pull_left A := repeat (rewrite <- (pull_right A) || rewrite <- (pull_right0 A)).
+
+Ltac pull_right A := repeat (rewrite (pull_right A) || rewrite (pull_right0 A)).
+
+Lemma pure_modus {A} {NA: NatDed A}{SA: SepLog A}{CA: ClassicalSep A}:
+  forall P Q,  P |-- Q -> pure Q -> P |-- Q && P.
+Proof.
+intros.
+apply andp_right; auto.
+Qed.
+
+Lemma derives_extract_prop {A} {NA: NatDed A}:
+  forall (P: Prop) (Q R: A), (P -> Q |-- R) ->  !!P && Q |-- R.
+Proof.
+ intros.
+ apply imp_andp_adjoint.
+ apply prop_left.
+ intros. apply imp_andp_adjoint. rewrite TT_andp. apply H; auto.
+Qed.
+
+Lemma derives_extract_prop' {A} {NA: NatDed A}:
+  forall (P: Prop) (Q R: A), (P -> Q |-- R) ->  Q && !!P|-- R.
+Proof.
+intros. rewrite andp_com. apply derives_extract_prop; auto.
+Qed.
+
+Lemma andp_assoc' {A}{NA: NatDed A}:
+  forall P Q R, Q && (P && R) = P && (Q && R).
+Proof. intros. rewrite andp_com. rewrite andp_assoc. f_equal. apply andp_com. 
+Qed.
+
+Definition corable {A} {NA: NatDed A}{SA: SepLog A} (P: A) : Prop :=
+ forall Q R, (P && Q) * R = P && (Q * R).
+
+Lemma corable_andp_sepcon1{A}  {NA: NatDed A}{SA: SepLog A} :
+   forall P Q R, corable P ->  (P && Q) * R = P && (Q * R).
+Proof. auto. Qed.
+
+Lemma corable_andp_sepcon2{A}  {NA: NatDed A}{SA: SepLog A} :
+   forall P Q R, corable P ->  (Q && P) * R = P && (Q * R).
+Proof.
+intros. rewrite andp_com. apply corable_andp_sepcon1. auto.
+Qed.
+
+Lemma corable_sepcon_andp1 {A}  {NA: NatDed A}{SA: SepLog A} :
+   forall P Q R, corable P ->  Q  * (P && R) = P && (Q * R).
+Proof.
+intros. rewrite sepcon_comm. rewrite corable_andp_sepcon1; auto. rewrite sepcon_comm; auto.
+Qed.
+
+Lemma corable_sepcon_andp2 {A}  {NA: NatDed A}{SA: SepLog A} :
+   forall P Q R, corable P ->  Q  * (R && P) = P && (Q * R).
+Proof.
+intros. rewrite sepcon_comm. rewrite andp_com. rewrite corable_andp_sepcon1; auto. rewrite sepcon_comm; auto.
+Qed.
+
+Lemma prop_corable{A}  {NA: NatDed A}{SA: SepLog A}: forall P, corable (!!P).
+Proof. unfold corable; intros.
+rewrite sepcon_andp_prop'.  auto.
+Qed.
+
+Hint Resolve @prop_corable : normalize.
+
+(* This hint doesn't work well, hence the extra clauses in normalize1 and normalize1_in *)
+Hint Rewrite @corable_andp_sepcon1 @corable_andp_sepcon2
+                    @corable_sepcon_andp1 @corable_sepcon_andp2 using solve [auto with normalize typeclass_instances].
+
+Ltac normalize1 := 
+         match goal with
+            | |- _ => contradiction
+            | |- context [@andp ?A (@LiftNatDed ?T ?B ?C) ?D ?E ?F] =>
+                      change (@andp A (@LiftNatDed T B C) D E F) with (D F && E F)
+            | |- context [@later ?A  (@LiftNatDed ?T ?B ?C) (@indir_ops _ _ (@LiftIndir ?X1 ?X2 ?X3 ?X4 ?X5)) ?D ?F] =>
+                   change (@later A  (@LiftNatDed T B C) (@indir_ops A (@LiftNatDed T B C) (@LiftIndir X1 X2 X3 X4 X5)) D F) 
+                     with (@later B C (@indir_ops B C X5) (D F))   
+            | |- context [@sepcon ?A (@LiftNatDed ?B ?C ?D) 
+                                                         (@LiftSepLog ?E ?F ?G ?H) ?J ?K ?L] =>
+                   change (@sepcon A (@LiftNatDed B C D) (@LiftSepLog E F G H) J K L)
+                      with (@sepcon C D H (J L) (K L))
+            | |- context [(?P && ?Q) * ?R] => rewrite (corable_andp_sepcon1 P Q R) by (auto with normalize)
+            | |- context [?Q * (?P && ?R)] => rewrite (corable_sepcon_andp1 P Q R) by (auto with normalize)
+            | |- context [(?Q && ?P) * ?R] => rewrite (corable_andp_sepcon2 P Q R) by (auto with normalize)
+            | |- context [?Q * (?R && ?P)] => rewrite (corable_sepcon_andp2 P Q R) by (auto with normalize)
+            | |-  derives ?A   _ => match A with 
+                          | context [ ((!! ?P) && ?Q) && ?R ] => rewrite (andp_assoc (!!P) Q R)
+                          | context [ ?Q && (!! ?P && ?R)] =>
+                                         match Q with !! _ => fail 2 | _ => rewrite (andp_assoc' (!!P) Q R) end
+                         end
+            | |- _ => progress  (autorewrite with normalize); auto with typeclass_instances
+            | |- _ = ?x -> _ => intro; subst x
+            | |- ?x = _ -> _ => intro; subst x
+            |  |- ?ZZ -> _ => match type of ZZ with 
+                                               | Prop => 
+                                                    let H := fresh in
+                                                       ((assert (H:ZZ) by auto; clear H; intros _) || intro H)
+                                               | _ => intros _
+                                              end             
+            | |- forall _, _ => let x := fresh "x" in (intro x; normalize1; try generalize dependent x)
+            | |- exp _ |-- _ => apply imp_extract_exp_left 
+            | |- !! _ && _ |-- _ => apply derives_extract_prop
+            | |- _ && !! _ |-- _ => apply derives_extract_prop'
+            | |- _ |-- !! (?x = ?y) && _ => 
+                            (rewrite prop_true_andp with (P:= (x=y))
+                                            by (unfold y; reflexivity); unfold y in *; clear y) ||
+                            (rewrite prop_true_andp with (P:=(x=y))
+                                            by (unfold x; reflexivity); unfold x in *; clear x)
+            | |- _ => solve [auto with typeclass_instances]
+            end.
+
+Ltac normalize1_in Hx := 
+             match type of Hx with
+                 | context [@andp ?A (@LiftNatDed ?T ?B ?C) ?D ?E ?F] =>
+                         change (@andp A (@LiftNatDed T B C) D E F) with (D F && E F)
+                 | context [@later ?A  (@LiftNatDed ?T ?B ?C) (@LiftIndir ?X1 ?X2 ?X3 ?X4 ?X5) ?D ?F] =>
+                    change (@later A  (@LiftNatDed T B C) (@LiftIndir X1 X2 X3 X4 X5) D F) 
+                     with (@later B C X5 (D F))   
+                 | context [@sepcon ?A (@LiftNatDed ?B ?C ?D) 
+                                                         (@LiftSepLog ?E ?F ?G ?H) ?J ?K ?L] =>
+                   change (@sepcon A (@LiftNatDed B C D) (@LiftSepLog E F G H) J K L)
+                      with (@sepcon C D H (J L) (K L))
+                | context [ !! ?P ] =>      
+                                    rewrite (true_eq P) in Hx by auto with typeclass_instances
+                | context [ !! ?P && ?Q ] =>  
+                                    rewrite (prop_true_andp P Q) in Hx by auto with typeclass_instances  
+                | context [(?P && ?Q) * ?R] => rewrite (corable_andp_sepcon1 P Q R) in Hx by (auto with normalize)
+                | context [?Q * (?P && ?R)] => rewrite (corable_sepcon_andp1 P Q R) in Hx by (auto with normalize)
+                | context [(?Q && ?P) * ?R] => rewrite (corable_andp_sepcon2 P Q R) in Hx by (auto with normalize)
+                | context [?Q * (?R && ?P)] => rewrite (corable_sepcon_andp2 P Q R) in Hx by (auto with normalize)
+                | _ => progress  (autorewrite with normalize in Hx); auto with typeclass_instances
+                end.
+
+Ltac normalize := repeat (auto with normalize; normalize1).
+
+Tactic Notation "normalize" "in" hyp(H) := repeat (normalize1_in H).
+
+Definition mark {A: Type} (i: nat) (j: A) := j.
+
+Lemma swap_mark1 {A} {NA: NatDed A}{SA: SepLog A}:
+  forall i j Pi Pj B, (i<j)%nat -> B * mark i Pi * mark j Pj = B * mark j Pj * mark i Pi.
+Proof.
+intros.
+repeat rewrite sepcon_assoc.
+f_equal.
+apply sepcon_comm.
+Qed.
+
+Lemma swap_mark0 {A} {NA: NatDed A}{SA: SepLog A}:
+  forall i j Pi Pj,  (i<j)%nat -> mark i Pi * mark j Pj = mark j Pj * mark i Pi.
+Proof.
+intros.
+apply sepcon_comm.
+Qed.
+
+Ltac select_left n :=
+  repeat match goal with 
+ | |- context [(_ * mark ?i _ * mark n _)] => 
+      rewrite (swap_mark1 i n); [ | solve [simpl; auto]]
+ | |- context [(mark ?i _ * mark n _)] => 
+      rewrite (swap_mark0 i n); [ | solve [simpl; auto]]
+end.
+Ltac select_all n := match n with 
+                                | O => idtac 
+                                | S ?n' => select_left n; select_all n' 
+                              end.
+Ltac markem n P := 
+   match P with 
+   | (?Y * ?Z) => 
+        (match goal with H: mark _ Z = Z |- _ => idtac end 
+        || assert (mark n Z = Z) by auto); markem (S n) Y
+   | ?Z =>  match goal with H: mark _ Z = Z |- _ => idtac end 
+                || assert (mark n Z = Z) by auto
+  end.
+
+Ltac prove_assoc_commut := 
+ clear;
+ try (match goal with |- ?F _ -> ?G _ => replace G with F; auto end);
+  (repeat rewrite <- sepcon_assoc; 
+   match goal with |- ?P = _ => markem O P end; 
+   let LEFT := fresh "LEFT" in match goal with |- ?P = _ => set (LEFT := P) end;
+  match goal with H: mark ?n _ = _ |- _ =>
+     repeat  match goal with H: mark ?n _ = ?P |- _ => rewrite <- H; clear H end;
+     select_all n;
+     reflexivity
+   end).
+
+Lemma test_prove_assoc_commut {T}{NA: NatDed T}{SA: SepLog T} : forall A B C D E : T,
+   D * E * A * C * B = A * B * C * D * E.
+Proof.
+intros.
+prove_assoc_commut.
+Qed.
+
+(***** contractiveness ******)
+
+Lemma later_fash1 {A} {NA: NatDed A}{IA: Indir A}:
+   forall P, |> # P |-- # |> P.
+Proof. intros. rewrite later_fash; auto.
+Qed.
+
+Lemma sub_later1 {A}  {NA: NatDed A}{IA: Indir A} : forall P Q,
+   |>(P >=> Q)  |--   |>P >=> |>Q.
+Proof.
+intros.
+rewrite later_fash. rewrite later_imp. auto.
+Qed.
+
+Lemma sub_later {A}  {NA: NatDed A}{IA: Indir A} : forall P Q,
+   |>(P >=> Q) = |>P >=> |>Q.
+Proof.
+intros.
+rewrite later_fash. rewrite later_imp. auto.
+Qed.
+
+Lemma eq_later1 {A} {NA: NatDed A}{IA: Indir A} : forall P Q,
+   |>(P <=> Q)  |--   |>P <=> |>Q.
+Proof.
+intros.
+rewrite later_fash.
+rewrite later_andp; repeat rewrite later_imp; repeat  rewrite fash_andp. auto.
+Qed.
+
+Lemma eq_later {A}  {NA: NatDed A}{IA: Indir A}  : forall P Q,
+    (|>(P <=> Q) = |>P <=> |>Q).
+Proof.
+intros.
+rewrite later_fash.
+rewrite later_andp; repeat rewrite later_imp; repeat  rewrite fash_andp. auto.
+Qed.
+
+Lemma sub_refl {A} {NA: NatDed A}{IA: Indir A}  : forall G P,
+  G |-- P >=> P.
+Proof.
+intros.
+rewrite <- (fash_triv G).
+apply @derives_trans with (#TT).
+apply fash_TT.
+apply fash_derives.
+apply imp_andp_adjoint.
+apply andp_left2; auto.
+Qed.
+
+Lemma sub_trans {A} {NA: NatDed A}{IA: Indir A}  : forall G P Q R,
+  G |-- P >=> Q ->
+  G |-- Q >=> R ->
+  G |-- P >=> R.
+Proof.
+intros.
+  apply @derives_trans with ((P >=> Q) && (Q >=> R)).
+ apply andp_right; auto.
+  clear.
+ rewrite <- fash_andp. apply fash_derives.
+ apply -> imp_andp_adjoint.
+ rewrite andp_com. rewrite <- andp_assoc.
+ eapply derives_trans; [ apply andp_derives | ].
+ apply modus_ponens. apply derives_refl. apply modus_ponens.
+Qed.
+
+Lemma sub_top {A} {NA: NatDed A}{IA: Indir A}  : forall G P,
+  G |-- P >=> TT.
+Proof.
+ intros. apply @derives_trans with (#TT).
+ apply fash_TT.
+ apply fash_derives. apply imp_andp_adjoint.
+ apply andp_left1; auto.
+Qed.
+
+Lemma sub_bot {A} {NA: NatDed A}{IA: Indir A}  : forall G P,
+  G |-- FF >=> P.
+Proof.
+ intros. apply @derives_trans with (#TT).
+ apply fash_TT.
+ apply fash_derives. apply imp_andp_adjoint.
+ apply andp_left2; apply FF_left.
+Qed.
+
+Lemma sub_andp {A} {NA: NatDed A}{IA: Indir A}  : forall G P P' Q Q',
+  G |-- P >=> P' ->
+  G |-- Q >=> Q' ->
+  G |-- P && Q >=> (P' && Q').
+Proof.
+ intros.
+ apply @derives_trans with ((P >=> P') && (Q >=> Q')).
+ apply andp_right; auto.
+ clear.
+ rewrite <- fash_andp. apply fash_derives.
+ apply -> imp_andp_adjoint.
+ apply @derives_trans with ((P && (P --> P')) && (Q && (Q --> Q'))).
+ repeat apply andp_right.
+ apply andp_left2. apply andp_left1; auto.
+ do 2 apply andp_left1; auto.
+ repeat apply andp_left2; auto.
+ apply andp_left1; apply andp_left2; auto.
+ apply andp_derives; apply modus_ponens.
+Qed.
+
+Lemma sub_imp {A} {NA: NatDed A}{IA: Indir A}  : forall G P P' Q Q',
+  G |-- P' >=> P ->
+  G |-- Q >=> Q' ->
+  G |-- (P --> Q) >=> (P' --> Q').
+Proof.
+ intros.
+ apply @derives_trans with ((P' >=> P) && (Q >=> Q')).
+ apply andp_right; auto.
+ clear.
+ rewrite <- fash_andp. apply fash_derives.
+ apply -> imp_andp_adjoint.
+ apply -> imp_andp_adjoint.
+ apply @derives_trans with (((P' && (P' --> P)) && (P --> Q)) && (Q --> Q')).
+ repeat apply andp_right.
+ apply andp_left2.  auto.
+ do 3 apply andp_left1; auto.
+ apply andp_left1. repeat apply andp_left2; auto.
+ apply andp_left1; apply andp_left1. apply andp_left2;  auto.
+ eapply derives_trans ; [eapply andp_derives | ].
+ eapply derives_trans ; [eapply andp_derives | ].
+ apply modus_ponens. apply derives_refl.
+ apply modus_ponens. apply derives_refl.
+ apply modus_ponens.
+Qed.
+
+Lemma sub_orp {A} {NA: NatDed A}{IA: Indir A}  : forall G P P' Q Q',
+  G |-- P >=> P' ->
+  G |-- Q >=> Q' ->
+  G |-- (P || Q) >=> (P' || Q').
+Proof.
+ intros.
+ eapply derives_trans; [ apply andp_right; [apply H | apply H0] | ].
+ clear.
+ rewrite <- fash_andp. apply fash_derives.
+ apply -> imp_andp_adjoint.
+rewrite andp_com. apply imp_andp_adjoint.
+apply orp_left; apply -> imp_andp_adjoint; [apply orp_right1 | apply orp_right2].
+ rewrite <- andp_assoc. apply andp_left1. apply modus_ponens.
+ rewrite (andp_com (_ --> _)).
+ rewrite <- andp_assoc. apply andp_left1. apply modus_ponens.
+Qed.
+
+Lemma sub_sub {A} {NA: NatDed A}{IA: Indir A}:
+  forall G (P Q R S: A), 
+   G |-- (R >=> P) ->
+   G |-- (Q >=> S) ->
+   G |-- (P >=> Q) >=> (R >=> S).
+Proof.
+ intros.
+ intros.
+ eapply derives_trans; [ apply andp_right; [apply H | apply H0] | ].
+ clear.
+ rewrite fash_triv.
+ apply -> (@imp_andp_adjoint Triv).
+ rewrite andp_assoc.
+ apply @derives_trans with ((R >=> P) && (P >=> S)).
+ apply andp_derives; auto.
+ apply sub_trans with Q. apply andp_left2; auto. apply andp_left1; auto.
+  apply sub_trans with P. apply andp_left1; auto. apply andp_left2; auto.
+Qed.
+
+Lemma allp_imp2_later_e2 {B}{A}{NA: NatDed A}{IA: Indir A}:
+   forall (P Q: B -> A) (y: B) ,
+      (All x:B, |> P x <=> |> Q x) |-- |> Q y >=> |> P y.
+Proof. 
+  intros. apply allp_left with y. repeat rewrite fash_andp. apply andp_left2; auto.
+Qed.
+
+Lemma allp_imp2_later_e1 {B}{A}{NA: NatDed A}{IA: Indir A}:
+   forall (P Q: B -> A) (y: B) ,
+      (All x:B, |> P x <=> |> Q x) |-- |> P y >=> |> Q y.
+Proof. 
+  intros. apply allp_left with y. repeat rewrite fash_andp. apply andp_left1; auto.
+Qed.
+
+Lemma prove_HOcontractive1 {A} {NA: NatDed A}{IA: Indir A}{RA: RecIndir A} : forall X F,
+  (forall P Q: X -> A,
+    (All x:X, |>(P x >=> Q x) |--
+        All x:X, F P x >=> F Q x)) ->
+   HOcontractive F.
+Proof.
+  unfold HOcontractive.
+  intros.
+  apply allp_right; intro v.
+  rewrite fash_andp.
+  apply andp_right.
+  specialize (H P Q).
+  eapply derives_trans; [ | eapply derives_trans ; [ apply H |] ].
+  apply allp_derives; intro x.
+  apply @later_derives. apply fash_derives. apply andp_left1. auto.
+  apply allp_left with v; auto.
+  specialize (H Q P).
+  eapply derives_trans; [ | eapply derives_trans ; [ apply H |] ].
+  apply allp_derives; intro x.
+  apply later_derives. apply fash_derives. apply andp_left2. auto.
+  apply allp_left with v; auto.
+Qed.
+
+Lemma prove_HOcontractive {A} {NA: NatDed A}{IA: Indir A}{RA: RecIndir A} : forall X F,
+  (forall (P Q: X -> A) (x: X),
+    (All x:X, (|> P x <=> |> Q x) |-- F P x >=> F Q x)) ->
+   HOcontractive F.
+Proof.
+  intros.
+  unfold HOcontractive.
+  intros.
+  apply allp_right; intro v.
+  rewrite fash_andp.
+  apply andp_right.
+  eapply derives_trans; [ | apply H].
+  apply allp_derives; intro x.
+  rewrite eq_later. auto.
+  eapply derives_trans; [ | apply H].
+  apply allp_derives; intro x.
+  rewrite eq_later. rewrite andp_com. auto.
+Qed.
+
+Lemma sub_sepcon {A} {NA: NatDed A}{IA: Indir A}{SA: SepLog A}{SI: SepIndir A} : forall G P P' Q Q',
+  G |-- P >=> P' ->
+  G |-- Q >=> Q' ->
+  G |-- P * Q >=> P' * Q'.
+Proof.
+Admitted.  (* prove this in SepIndir? *)
+
+Ltac sub_unfold := 
+   match goal with 
+    | |- _ |-- ?A _ >=> ?A _ => unfold A 
+    | |- _ |-- ?A _ _ >=> ?A _ _ => unfold A 
+    | |- _ |-- ?A _ _ _ >=> ?A _ _ _ => unfold A 
+    | |- _ |-- ?A _ _ _ _ >=> ?A _ _ _ _ => unfold A 
+    | |- _ |-- ?A _ _ _ _ _ >=> ?A _ _ _ _ _ => unfold A 
+    | v: _ |- _ => destruct v
+   end.
+
+Hint Extern 2 (_ |-- _ >=> _) => sub_unfold : contractive.
+
+Hint Resolve @prove_HOcontractive 
+  @sub_allp @sub_imp @sub_refl @sub_exp @sub_andp @sub_orp @sub_sub 
+  @sub_sepcon (* NOTE: This hint fails to work unless fully instantiated, for some reason;
+                             so the client must re-do the sub_sepcon hint *)
+  @allp_imp2_later_e1 @allp_imp2_later_e2 : contractive.
+
+(*Lemma Rec_sub {A} {NA: NatDed A}{IA: Indir A}{RA: RecIndir A} : forall G
+  (F   : A -> A -> A)
+  (HF1 : forall X, contractive (F X))
+  (HF2 : forall R P Q, P >=> Q |-- F P R >=> F Q R)
+  (HF3 : forall P Q X, |>(P >=> Q) |-- F X P >=> F X Q),
+  forall P Q,
+    G |-- P >=> Q ->
+    G |-- Rec (F P) >=> Rec (F Q).
+*)
+
+Lemma HORec_sub {A}  {NA: NatDed A}{IA: Indir A}{RA: RecIndir A} : forall G B
+  (F : A -> (B -> A) -> B -> A)
+  (HF1 : forall X, HOcontractive (F X))
+  (HF2 : forall R a P Q, P >=> Q |-- F P R a >=> F Q R a)
+  (HF3 : forall P Q X, All b:B, |>(P b >=> Q b) |-- All b:B, F X P b >=> F X Q b),
+  forall P Q,
+    G |-- P >=> Q ->
+    G |-- All b:B, HORec (F P) b >=> HORec (F Q) b.
+Proof.
+  intros.
+  apply @derives_trans with (P>=>Q); auto.
+  clear G H.
+  apply goedel_loeb.
+  apply allp_right; intro b.
+  rewrite HORec_fold_unfold by auto.
+  pose proof (HORec_fold_unfold _ _ (HF1 P)). 
+  pose proof (HORec_fold_unfold _ _ (HF1 Q)). 
+  set (P' := HORec (F P)) in *.
+  set (Q' := HORec (F Q)) in *.
+  rewrite <- H.
+  specialize (HF3 P' Q' P).
+  rewrite later_allp.
+ eapply derives_trans; [apply andp_derives ; [apply derives_refl | apply HF3] | ].
+  specialize (HF2 Q' b P Q). rewrite <- H0 in HF2.
+ rewrite <- H in *.
+  apply sub_trans with  (F P Q' b).
+  apply andp_left2.  apply allp_left with b; auto.
+  apply andp_left1; auto.
+Qed.
+
+(*
+Lemma Rec_contractive {A}  {NA: NatDed A}{IA: Indir A}{RA: RecIndir A}  : forall
+  (F   : A -> A -> A)
+  (HF1 : forall X, contractive (F X))
+  (HF2 : forall R, contractive (fun X => F X R)),
+  contractive (fun X => Rec (F X)).
+
+Lemma Rec_nonexpansive {A} `{ageable A} : forall
+  (F   : pred A -> pred A -> pred A)
+  (HF1 : forall X, contractive (F X))
+  (HF2 : forall R, nonexpansive (fun X => F X R)),
+  nonexpansive (fun X => Rec (F X)).
+
+
+Lemma HORec_contractive {A} `{ageable A} : forall B
+  (F : pred A -> (B -> pred A) -> B -> pred A)
+  (HF1 : forall X, HOcontractive (F X))
+  (HF2 : forall R a, contractive (fun X => F X R a)),
+  forall a, contractive (fun X => HORec (F X) a).
+
+Lemma HORec_nonexpansive {A} `{ageable A} : forall B
+  (F : pred A -> (B -> pred A) -> B -> pred A)
+  (HF1 : forall X, HOcontractive (F X))
+  (HF2 : forall R a, nonexpansive (fun X => F X R a)),
+  forall a, nonexpansive (fun X => HORec (F X) a).
+*)
+
+(****** End contractiveness *****)
+
