veric/expr.v
@@ -1,4 +1,4 @@
-Require Export msl.msl_standard.
+Require Import msl.msl_standard.
 Require Import veric.base.
 Require Import veric.Address.
 Require Import msl.rmaps.
